Add Hadamard-Hadamard simplification

Main.lean
@@ -37,3 +37,17 @@ theorem doPpmSimp : piPiMinus ≈z ppmSimplified := by
   zx_rfl
 
 #print axioms doPpmSimp
+
+def zHadHad : ZXDiagram :=
+  ZXDiagram.ofList
+    [.input 0, .spider .Z ⟨1, 1⟩, .hadamard, .hadamard, .output 0]
+    [⟨0, 1⟩, ⟨1, 2⟩, ⟨2, 3⟩, ⟨3, 4⟩]
+
+def zHadHadSimplified : ZXDiagram :=
+  { nodes := [some (.input 0), some (.spider .Z ⟨1, 1⟩), none, none, some (.output 0)]
+    edges := [⟨0, 1⟩, ⟨1, 4⟩] }
+
+theorem dozHadHadSimp : zHadHad ≈z zHadHadSimplified := by
+  zx_show
+  zx_hadamard_hadamard 2 3
+  zx_rfl
