ZxLean/Rules/HadamardHadamard.lean
@@ -1,0 +1,39 @@
+import ZxLean.Axioms
+import ZxLean.Tactics
+
+open Lean Elab Tactic Meta
+
+def ZXDiagram.hadamardHadamard (d: ZXDiagram) (a b : NodeId) : Except String ZXDiagram := do
+  let nodeA ← (d.getNode? a).toExcept s!"Node {a} not found"
+  let nodeB ← (d.getNode? b).toExcept s!"Node {b} not found"
+  unless nodeA.isHadamard do throw s!"Node {a} is not a Hadamard"
+  unless nodeB.isHadamard do throw s!"Node {b} is not a Hadamard"
+  unless d.connected a b do throw s!"Nodes {a} and {b} are not connected"
+  let aNeighbors := d.neighbors a |>.filter (· != b)
+  let bNeighbors := d.neighbors b |>.filter (· != a)
+  unless aNeighbors.length == 1 do throw s!"Node {a} has {aNeighbors.length} neighbours other than node {b} (should be 1)"
+  unless bNeighbors.length == 1 do throw s!"Node {b} has {aNeighbors.length} neighbours other than node {a} (should be 1)"
+  let n0 ← (aNeighbors[0]?).toExcept s!"Node {a} neighbour not found"
+  let n1 ← (bNeighbors[0]?).toExcept s!"Node {b} neighbour not found"
+  let d := d.removeEdgesOf a
+  let d := d.removeNode a
+  let d := d.removeEdgesOf b
+  let d := d.removeNode b
+  let d := { d with edges := d.edges ++ [Edge.mk n0 n1] }
+  return d.normalize
+
+namespace ZxLean
+
+axiom ZXDiagram.hadamardHadamard_sound (d : ZXDiagram) (a b : NodeId) (d' : ZXDiagram) :
+  d.hadamardHadamard a b = .ok d' → d ≈z d'
+
+/-- Remove two connected degree-2 Hadamards. Shows the resulting diagram. -/
+syntax "zx_hadamard_hadamard" num num : tactic
+
+elab_rules : tactic
+  | `(tactic| zx_hadamard_hadamard $a $b) =>
+    applyRewrite a "Hadamard Hadamard"
+      ``ZXDiagram.hadamardHadamard ``ZXDiagram.hadamardHadamard_sound
+      #[mkNatLit a.getNat, mkNatLit b.getNat]
+
+end ZxLean
